FiatFormal/Language/SubstExistential.v
@@ -1,6 +1,71 @@
 
+Require Import FiatFormal.Language.SubstExpExp.
 Require Import FiatFormal.Language.TyJudge.
 Require Import FiatFormal.Language.SubstTypeType.
+
+Theorem subst_exp_prog_ix :
+  forall ke te t1 ix p t2 s,
+    get ix te = Some t1
+    -> TYPE ke (delete ix te) s t1
+    -> TYPEPROG ke te p t2
+    -> TYPEPROG ke (delete ix te) (substXP ix s p) t2.
+Proof.
+  intros. gen s ix t1.
+  induction H1; intros.
+  Case "PLet".
+  invert H; intros; subst; simpl.
+  apply TYLet.
+  (* prove A generalized *)
+  apply TYADT; try assumption.
+  eapply subst_value_value_ix; first [ eassumption; assumption ].
+  (* prove B generalized *)
+  unfold liftTE in *.
+  rewrite map_delete.
+  rewrite delete_rewind.
+  eapply IHTYPEPROG; simpl.
+  apply get_map.
+  eassumption.
+  apply type_tyenv_weaken.
+  rewrite <- map_delete.
+  pose proof type_kienv_weaken.
+  unfold liftTE in H.
+  apply H. assumption.
+  Case "PExp".
+  apply TYExp.
+  eapply subst_value_value_ix; first [ eassumption |  assumption].
+Qed.
+
+Theorem subst_exp_prog
+  : forall ke te t1 p t2 s,
+    TYPEPROG ke (te :> t1) p t2
+    -> TYPE ke te s t1
+    -> TYPEPROG ke te (substXP 0 s p) t2.
+Proof.
+  intros.
+  assert (te = delete 0 (te :> t1)). auto.
+  rewrite H1.
+  eapply subst_exp_prog_ix; simpl; eauto.
+Qed.
+
+
+Theorem subst_type_prog
+  : forall ke te X S p t,
+    TYPEPROG (ke :> X) te p t
+    -> KIND ke S KStar
+    -> TYPEPROG ke (substTE 0 S te) (substTP 0 S p) (substTT 0 S t).
+Proof.
+Admitted.
+
+Theorem subst_ADT_prog :
+  forall X r t1 t2 x p,
+    TYPEPROG (nil :> X) (nil :> t1) p t2
+    -> TYPE nil nil x (substTT 0 r t1)
+    -> TYPEPROG nil nil (substXP 0 x (substTP 0 r p)) (substTT 0 r t2).
+Proof.
+Admitted.
+
+(* ------------------------------------------------------------ *)
+
 
 (* Substitution lemma for substituting ADT contents into ADTs.
    This is unnecessary if we further restrict ADTs such that method bodies may
@@ -11,17 +76,23 @@ Require Import FiatFormal.Language.SubstTypeType.
    to the result type.
  *)
 
-Theorem subst_exist_exp
-  : forall ke te t1 kr tr x1 t2 x,
-    KIND ke tr kr
-    -> TYPE ke te x1 (substTT 0 tr t1)
-    -> TYPE (ke :> kr) (te :> t1) x t2
-    -> TYPE ke te (substTX 0 tr (substXX 0 x1 x)) t2.
-Proof.
-  intros. gen ke te t1 kr tr x1 t2.
-  induction x; intros; simpl.
-  Case "XVar".
-  lift_cases.
+(* Theorem subst_exist_exp *)
+(*   : forall ke te t1 kr k2 tr x1 t2 x, *)
+(*     KIND ke tr kr *)
+(*     -> KIND ke t2 k2 *)
+(*     -> TYPE ke te x1 (substTT 0 tr t1) *)
+(*     -> TYPE (ke :> kr) (te :> t1) x t2 *)
+(*     -> TYPE ke te (substTX 0 tr (substXX 0 x1 x)) t2. *)
+(* Proof. *)
+(*   intros. gen ke te t1 kr k2 tr x1 t2. *)
+(*   induction x; intros. *)
+(*   Case "XVar". *)
+(*   simpl. *)
+(*   lift_cases. *)
+(*   inverts H2. simpl in *. *)
+(*   norm_inverts_option. *)
+(* Admitted. *)
+
 
 (* Substitution lemma for substituting ADT contents into ADTs.
    This is unnecessary if we further restrict ADTs such that method bodies may
@@ -33,14 +104,17 @@ Proof.
  *)
 
 (* Not clear that this particular statement is what I want *)
-Theorem subst_exist_adt
-  : forall ke te t1 kr tr x1 t2 ad,
-    KIND ke tr kr (* well-kinded rep type *)
-    -> TYPE ke te x1 (substTT 0 tr t1) (* existential well-typed *)
-    -> TYPEADT (ke :> kr) (te :> t1) ad t2
-    -> TYPEADT ke te (substTADT 0 tr (substXADT 0 x1 ad)) t2.
-Proof.
-Abort.
+(* Theorem subst_exist_adt *)
+(*   : forall ke te t1 kr tr x1 t2 ad, *)
+(*     KIND ke tr kr (* well-kinded rep type *) *)
+(*     -> TYPE ke te x1 (substTT 0 tr t1) (* existential well-typed *) *)
+(*     -> TYPEADT (ke :> kr) (te :> t1) ad t2 *)
+(*     -> TYPEADT ke te (substTADT 0 tr (substXADT 0 x1 ad)) t2. *)
+(* Proof. *)
+(*   intros. gen ke te t1 kr tr x1 t2. *)
+(*   induction ad; intros. *)
+(* Admitted. *)
+
 
 (* Main substitution lemma for substituting ADT contents into program.
    If an ADT's methods implement their abstract interfaces,
@@ -52,26 +126,32 @@ Abort.
    to the result type.
  *)
 
-Theorem subst_exist_prog
-  : forall ke te t1 kr tr x1 t2 p,
-    KIND ke tr kr (* well-kinded rep type *)
-    -> TYPE ke te x1 (substTT 0 tr t1) (* existential well-typed *)
-    -> TYPEPROG (ke :> kr) (te :> t1) p t2 (* program well-typed with extended contexts *)
-    -> TYPEPROG ke te (substTP 0 tr (substXP 0 x1 p)) t2.
-Proof.
-Abort.
+(* Theorem subst_exist_prog *)
+(*   : forall ke te t1 kr tr x1 t2 p, *)
+(*     KIND ke tr kr (* well-kinded rep type *) *)
+(*     -> TYPE ke te x1 (substTT 0 tr t1) (* existential well-typed *) *)
+(*     -> TYPEPROG (ke :> kr) (te :> t1) p t2 (* program well-typed with extended contexts *) *)
+(*     -> TYPEPROG ke te (substTP 0 tr (substXP 0 x1 p)) t2. *)
+(* Proof. *)
+(*   intros. *)
+(*   gen ke te t1 kr tr x1 t2. *)
+(*   induction p; intros. *)
+(*   Case "PLet". *)
+(*   simpl; destruct a; simpl. *)
+(*   eapply TYLet. *)
+(* Abort. *)
 
-Theorem subst_exist_prog_ix
-  : forall ix ix' ke te k t tr t2 x1 p,
-    get ix ke = Some k
-    -> get ix' te = Some t
-    -> KIND (delete ix ke) tr k
-    -> TYPEPROG ke te p t2
-    (* NOTE: the liftTT-ing for taur below shouldn't be necessary, just not sure where the simple condition on rep types should ultimately be stated *)
-    -> TYPE (delete ix ke) (delete ix' te) x1 (substTT 0 tr t)
-    -> TYPEPROG (delete ix ke) (delete ix' te) (substTP 0 tr (substXP 0 x1 p)) t2.
-Proof.
-Abort.
+(* Theorem subst_exist_prog_ix *)
+(*   : forall ix ix' ke te k t tr t2 x1 p, *)
+(*     get ix ke = Some k *)
+(*     -> get ix' te = Some t *)
+(*     -> KIND (delete ix ke) tr k *)
+(*     -> TYPEPROG ke te p t2 *)
+(*     (* NOTE: the liftTT-ing for taur below shouldn't be necessary, just not sure where the simple condition on rep types should ultimately be stated *) *)
+(*     -> TYPE (delete ix ke) (delete ix' te) x1 (substTT 0 tr t) *)
+(*     -> TYPEPROG (delete ix ke) (delete ix' te) (substTP 0 tr (substXP 0 x1 p)) t2. *)
+(* Proof. *)
+(* Abort. *)
   (* intros. *)
   (* gen ix ix' ke te k. (* TODO: ask why gen fails with all idents in a single invocation *) *)
   (* gen t tr t2 x1. *)
