FiatFormal/Language/Ty.v
@@ -6,7 +6,7 @@ Require Export FiatFormal.Language.Ki.
 Inductive ty  : Type :=
  | TCon    : nat -> ty             (* Data type constructor. *)
  | TVar    : nat -> ty             (* deBruijn index. *)
- | TForall : ty  -> ty           (* Type variable binding. *)
+ (* | TForall : ty  -> ty           (* Type variable binding. *) *)
  | TFun    : ty  -> ty -> ty     (* Function type constructor. *)
 
  | TExists : ty -> ty.
@@ -23,7 +23,7 @@ Fixpoint wfT (ke: kienv) (tt: ty) : Prop :=
  match tt with
  | TCon _     => True
  | TVar i     => exists k, get i ke = Some k
- | TForall t  => wfT (ke :> KStar) t
+ (* | TForall t  => wfT (ke :> KStar) t *)
  | TFun t1 t2 => wfT ke t1 /\ wfT ke t2
 
  (* | TNProd ts      => True *)
@@ -53,8 +53,8 @@ Fixpoint liftTT (d: nat) (tt: ty) : ty :=
        then TVar (S ix)
        else tt
 
-  |  TForall t
-     => TForall (liftTT (S d) t)
+  (* |  TForall t *)
+  (*    => TForall (liftTT (S d) t) *)
 
   |  TFun t1 t2
      => TFun    (liftTT d t1) (liftTT d t2)
@@ -87,8 +87,8 @@ Fixpoint substTT (d: nat) (u: ty) (tt: ty) : ty
        | _  => TVar  ix
        end
 
-    |  TForall t
-    => TForall (substTT (S d) (liftTT 0 u) t)
+    (* |  TForall t *)
+    (* => TForall (substTT (S d) (liftTT 0 u) t) *)
 
     |  TFun t1 t2
        => TFun (substTT d u t1) (substTT d u t2)
@@ -112,10 +112,10 @@ Proof.
   simpl.
   repeat (unfold liftTT; lift_cases; intros); burn.
 
- Case "TForall".
-  simpl.
-  assert (S (n + n') = (S n) + n'). omega. rewrite H.
-  rewrite IHt. auto.
+ (* Case "TForall". *)
+ (*  simpl. *)
+ (*  assert (S (n + n') = (S n) + n'). omega. rewrite H. *)
+ (*  rewrite IHt. auto. *)
 
  Case "TFun".
  simpl. apply f_equal2; auto.
@@ -147,9 +147,9 @@ Proof.
    fbreak_nat_compare; intros;
    burn.
 
- Case "TForall".
-  simpl.
-  rewrite IHt1. auto.
+ (* Case "TForall". *)
+ (*  simpl. *)
+ (*  rewrite IHt1. auto. *)
 
  Case "TFun".
   simpl.
@@ -176,10 +176,10 @@ Proof.
           try lift_cases; try intros);
    burn.
 
- Case "TForall".
-  simpl.
-  rewrite (IHt1 (S n) n'). simpl.
-  rewrite (liftTT_liftTT 0 n). auto.
+ (* Case "TForall". *)
+ (*  simpl. *)
+ (*  rewrite (IHt1 (S n) n'). simpl. *)
+ (*  rewrite (liftTT_liftTT 0 n). auto. *)
 
  Case "TFun".
   simpl.
@@ -207,10 +207,10 @@ Proof.
          ; try lift_cases; try fbreak_nat_compare
          ; intros); burn.
 
- Case "TForall".
-  simpl. f_equal.
-  rewrite (IHt1 (S n) n'). f_equal.
-   simpl. rewrite (liftTT_liftTT 0 (n + n')). auto.
+ (* Case "TForall". *)
+ (*  simpl. f_equal. *)
+ (*  rewrite (IHt1 (S n) n'). f_equal. *)
+ (*   simpl. rewrite (liftTT_liftTT 0 (n + n')). auto. *)
 
  Case "TFun".
   simpl. f_equal.
@@ -238,11 +238,11 @@ Proof.
   repeat (simpl; fbreak_nat_compare); try burn.
   rewrite substTT_liftTT. auto.
 
- Case "TForall".
-  simpl. f_equal.
-  rewrite (IHt1 (S n) m). f_equal.
-   simpl. rewrite (liftTT_substTT 0 (n + m)). auto.
-   simpl. rewrite (liftTT_liftTT 0 n). auto.
+ (* Case "TForall". *)
+ (*  simpl. f_equal. *)
+ (*  rewrite (IHt1 (S n) m). f_equal. *)
+ (*   simpl. rewrite (liftTT_substTT 0 (n + m)). auto. *)
+ (*   simpl. rewrite (liftTT_liftTT 0 n). auto. *)
 
  Case "TFun".
   simpl. f_equal.
