FiatFormal/PMKTactics.v
@@ -1,9 +1,21 @@
 Require Import FiatFormal.Tactics.LibTactics.
+(* Require Import Coq.Init.Nat. *)
 
-Ltac ex_spec :=
-  match goal with
-  | [ H1 : ?P, H2 : (exists _, ?A) -> ?B |- _ ] => destruct H2; eexists; eassumption
-  end.
+(* Print Implicit ex_intro. *)
 
-Tactic Notation "gen" ident(I1) ident(I2) ident(I3) ident(I4) ident(I5) ident(I6) ident(I7) ident(I8) ident(I9) ident(I10) :=
-  gen I10; gen I9; gen I8; gen I7; gen I6; gen I5; gen I4; gen I3; gen I2; gen I1.
+(* Ltac ex_spec := *)
+(*   match goal with *)
+(*   | [ H1 : ?B, H2 : (exists n, @?A n) -> ?R |- _ ] => pose proof (H2 (ex_intro _ _ H1)) *)
+(*   end. *)
+
+(* (* Ltac ex_spec' := *) *)
+(* (*   match goal with *) *)
+(* (*   | [ H1 :  ] *) *)
+
+(* Lemma foo : 3 < 6 -> forall n, even n = true -> ((exists m, even m = true) -> True) -> False. *)
+(* Proof. *)
+(*   intros. *)
+(*   ex_spec. *)
+
+(* Tactic Notation "gen" ident(I1) ident(I2) ident(I3) ident(I4) ident(I5) ident(I6) ident(I7) ident(I8) ident(I9) ident(I10) := *)
+(*   gen I10; gen I9; gen I8; gen I7; gen I6; gen I5; gen I4; gen I3; gen I2; gen I1. *)
